theories/Nominal.v
@@ -10,7 +10,7 @@ Section Nominal.
   Class Nominal `{Spt : Support X}: Prop := {
     nperm :> Perm X;
     support_spec : ∀ (x: X) (a b: name),
-        a ∉ (support x) → b ∉ (support x) → [(a,b)] • x ≡@{X} x
+        a ∉ (support x) → b ∉ (support x) → ⟨a,b⟩ • x ≡@{X} x
 }.
 End Nominal.
 Arguments support_spec {_ PrA _ _ Nmn} : rename.
