theories/ProperFun.v
@@ -1,0 +1,58 @@
+From Nominal Require Import Perm.
+
+Section ProperPermFun.
+  Context (A B: Type) `{Perm A, Perm B}.
+  
+  Record proper_perm_fun : Type := ProperPermFun {
+    fproper :> A → B;
+(*  f_to : Perm A;
+    f_from : Perm B; *)
+    fproper_spec : Proper ((≡@{A}) ⟹ (≡@{B})) fproper
+  }.
+End ProperPermFun.
+
+Arguments ProperPermFun {_ _ _ _} _ {_}.
+Existing Instance fproper_spec.
+
+Notation "'λp' x .. y , t" :=
+  (@ProperPermFun _ _ _ _ (λ x, .. (@ProperPermFun _ _ _ _ (λ y, t) _) ..) _)
+  (at level 200, x binder, y binder, right associativity).
+  
+Notation " A ⇥ B " := (proper_perm_fun A B) (at level 99, B at level 200, right associativity).
+
+Section proper_perm_fun.
+  Context `{Perm A, Perm B}.
+  
+  #[global] Instance perm_fun_proper (f: A ⇥ B): Proper ((≡@{A}) ⟹ (≡@{B})) f.
+  Proof. apply fproper_spec. Qed.
+
+  #[global] Instance perm_fun_proper_equiv: Equiv (A ⇥ B) := 
+    λ f g, ∀ (a : A), f a ≡@{B} g a.
+
+  #[global] Instance perm_fun_proper_equivalence : Equivalence perm_fun_proper_equiv.
+  Proof. split; repeat intro; [reflexivity | symmetry | etransitivity]; eauto. Qed.
+
+  #[global] Instance: Proper (perm_fun_proper_equiv ⟹ (≡@{A}) ⟹ (≡@{B})) (fproper A B).
+  Proof. repeat intro; rewrite H4; auto. Qed.
+
+  #[global,refine] Instance perm_fun_proper_act : PermAct (A ⇥ B) :=
+    λ p (f: A ⇥ B), (λp (a : A), p • f(-p • a)).
+  Proof.
+    - assumption.
+    - assumption.
+    - typeclasses eauto.
+    - repeat intro; apply gact_proper.
+      + reflexivity.
+      + apply fproper_spec; apply gact_proper; auto.  
+  Defined. 
+
+  #[global] Instance perm_fun_proper_perm: Perm (A ⇥ B).
+  Proof. split.
+    - apply perm_fun_proper_equivalence.
+    - intros ? ? EE f g EF ?; simpl; rewrite EE, EF; auto. 
+    - unfold equiv, perm_fun_proper_equiv; intros; simpl;
+        rewrite gact_id, grp_inv_neutral, gact_id; reflexivity.
+    - unfold equiv, perm_fun_proper_equiv; intros; simpl;
+        rewrite <-perm_op_inv, 2!gact_compat; reflexivity.
+  Qed.
+End proper_perm_fun.
